refactor so helpers are in a separate file, adequacy is in a separate file. add global minit variable to quantify escape hatch ind memories. add axiom about memory never evaluating to locations. prove lemma 5! also figure out that we need to prove lemma 4 (type preservation)

ImpE.v
@@ -179,6 +179,8 @@ Section Semantics.
   Definition mem : Type := memory val.
   Definition loc_mode : Type := location -> mode.
 
+  Axiom No_Pointers : forall (m: mem) l l', m l <> Vloc l'.
+
   Inductive event : Type :=
   | Decl : exp -> mem -> event
   | Mem : mem -> event
@@ -353,7 +355,7 @@ Section Typing.
        | Typ : base_type -> sec_level -> type.
 
   Definition context : Type := var -> option type.
-  Global Parameter Loc_Contxt : location -> option (type * ref_type).
+  Parameter Loc_Contxt : location -> option (type * ref_type).
   
   Lemma var_in_dom_dec : forall (G : context) x, {exists t, G x = Some t} + {G x = None}.
   Proof.
@@ -408,26 +410,25 @@ Section Typing.
   Definition is_var_low_context (G: context) : Prop :=
     forall_dom G (fun _ t => let (_, p) := t in p = L).
 
-  Definition all_loc_immutable (e: exp) : Prop :=
-    forall_subexp e (fun e =>
-                       match e with
-                       | Eloc n => forall t rt,
-                           Loc_Contxt n = Some (t, rt) ->
-                           rt = Immut
-                       | _ => True
-                       end).
-
-  Definition loc_in_exp (e: exp) (l: location) : Prop :=
-    forall_subexp e (fun e =>
-                       match e with
-                       | Eloc l => True
-                       | _ => False
-                       end).
+  Function loc_in_exp (e: exp) (l: location) : Prop :=
+    match e with
+    | Eloc l' => l = l'
+    | Ederef e' => loc_in_exp e' l
+    | Ebinop e1 e2 _ => loc_in_exp e1 l \/ loc_in_exp e2 l
+    | _ => False
+    end.
 
   Definition exp_locs_immutable (e: exp) :=
     forall_subexp e (fun e =>
                        match e with
                        | Eloc n => set_In n (immutable_locs g0)
+                       | _ => True
+                       end).
+
+  Definition exp_no_nested_derefs (e: exp) :=
+    forall_subexp e (fun e =>
+                       match e with
+                       | Ederef (Ederef e') => False
                        | _ => True
                        end).
 
