ImpE2Adequacy.v
@@ -1,0 +1,400 @@
+Require Import Bool Arith List Omega ListSet.
+Require Import Recdef Morphisms.
+Require Import Program.Tactics.
+Require Import Relation_Operators.
+Require FMapList.
+Require FMapFacts.
+Require Import Classical.
+Require Import Coq.Classes.RelationClasses.
+Require Import OrderedType OrderedTypeEx DecidableType.
+Require Import Coq.Logic.FunctionalExtensionality.
+Require Import Sorting.Permutation.
+Require Import Coq.Sets.Ensembles.
+Import ListNotations.
+Require Import Common.
+Require Import ImpE.
+Require Import ImpE2.
+Require Import ImpE2Helpers.
+
+Ltac unfold_cfgs :=
+  unfold ccfg_update_reg2 in *;
+  unfold ccfg_to_ecfg2 in *;
+  unfold ccfg_reg in *;
+  unfold ccfg_mem in *;
+  unfold ccfg_com in *;
+  unfold ccfg_reg2 in *;
+  unfold ccfg_mem2 in *;
+  unfold ccfg_com2 in *;
+  unfold ecfg_exp2 in *;
+  unfold ecfg_reg2 in *;
+  unfold ecfg_update_exp2 in *;
+  unfold ccfg_update_com2 in *;
+  unfold ccfg_update_mem2 in *;
+  unfold ccfg_update_mem in *;
+  unfold ccfg_update_reg in *;
+  unfold ccfg_update_com in *;
+  unfold ccfg_to_ecfg in *;
+  unfold project_ccfg.
+
+(*******************************************************************************
+*
+* Soundness
+*
+*******************************************************************************)
+Section Soundness.
+  Lemma impe2_exp_sound : forall md d e r m v is_left,
+      estep2 md d (e, r, m) v ->
+      estep md d (e, project_reg r is_left, project_mem m is_left) (project_value v is_left).
+  Proof.
+    intros.
+    remember (e, r, m) as ecfg.
+    generalize dependent e.
+    induction H; intros; try rewrite Heqecfg in H; simpl in *; try rewrite H.
+    1-3: constructor; simpl; auto.
+    - apply Estep_var with (x:=x); auto; subst; apply project_comm_reg.
+    - destruct_conjs.
+      apply contains_nat_project_nat with (is_left := is_left) in H2; destruct H2.
+      apply contains_nat_project_nat with (is_left := is_left) in H3; destruct H3.
+      pose (project_value_apply_op op v1 v2 x x0 is_left H2 H3); rewrite e0.
+      apply Estep_binop with (e1:=e1) (e2:=e2); simpl; auto;
+        [rewrite <- H2; apply (IHestep2_1 e1) | rewrite <- H3; apply (IHestep2_2 e2)];
+        rewrite Heqecfg; unfold ecfg_update_exp2; auto.
+    - inversion H; subst.
+      apply Estep_deref with (e:=e) (l:=l) (m:=project_mem m0 is_left)
+                                    (r:=project_reg r0 is_left); simpl; auto.
+  Qed.
+
+  Lemma impe2_sound : forall md d c r m r' m' t is_left,
+    cstep2 md d (c, r, m) (r', m') t ->
+    cstep md d (project_ccfg (c, r, m) is_left)
+          (project_reg r' is_left, project_mem m' is_left) (project_trace t is_left).
+  Proof.
+    intros.
+    remember (c, r, m) as ccfg.
+    remember (r', m') as cterm.
+    generalize dependent r'.
+    generalize dependent m'.
+    generalize dependent c.
+    induction H; intros; try rewrite Heqccfg in H, Heqcterm; simpl in *; inversion Heqcterm; subst.
+    - constructor; auto.
+    - apply impe2_exp_sound with (is_left:=is_left) in H0.
+      apply Cstep_assign with (x:=x) (e:=e) (v := project_value v is_left); auto.
+      unfold ccfg_to_ecfg; simpl in *; auto.
+      apply project_update_comm_reg.
+    - apply impe2_exp_sound with (is_left:=is_left) in H1.
+      apply Cstep_declassify with (x:=x) (e:=e) (v :=(project_value v is_left)); auto.
+      apply project_update_comm_reg.
+    - apply impe2_exp_sound with (is_left:=is_left) in H0.
+      apply impe2_exp_sound with (is_left:=is_left) in H1.
+      apply Cstep_update with (e1 := e1) (e2 := e2) (l := l) (v := project_value v is_left); auto.
+      now apply project_update_comm_mem.
+    - apply impe2_exp_sound with (is_left:=is_left) in H0; simpl in *.
+      apply Cstep_output with (e := e); auto.
+      destruct sl; auto.
+    - apply impe2_exp_sound with (is_left:=is_left) in H0; simpl in *.
+      apply Cstep_call with (e := e) (c := c); auto.
+      apply IHcstep2 with (c1 := c); auto.
+    - apply impe2_exp_sound with (is_left := is_left) in H0; simpl in *;
+        apply project_merge_inv_reg in H3; apply project_merge_inv_mem in H4.
+      destruct_conjs; subst.
+      destruct is_left;
+        [apply Cstep_call with (e:=e) (c:=c1) | apply Cstep_call with (e:=e) (c:=c2)]; auto;
+      unfold ccfg_update_com; simpl; rewrite project_merge_inv_trace; auto.
+    - apply Cstep_enclave with (enc := enc) (c := c); auto.
+      apply IHcstep2 with (c1 := c); auto.
+    - apply Cstep_seq_nil; auto. 
+    - apply Cstep_seq_hd with (hd:=hd) (tl:=tl)
+                                       (r:=(project_reg r0 is_left))
+                                       (m:=(project_mem m0 is_left))
+                                       (tr:=(project_trace tr is_left))
+                                       (tr':=(project_trace tr' is_left)); auto.
+      apply IHcstep2_1 with (c0:=hd); auto.
+      apply IHcstep2_2 with (c:=Cseq tl); auto.
+      admit.
+      (* XXX: getting stuck with a weird induction hypothesis... maybe generalizing wrong *)
+      now apply project_app_trace.
+    - apply impe2_exp_sound with (is_left := is_left) in H0; simpl in *.
+      apply Cstep_if with (e:=e) (c1:=c1) (c2:=c2); auto.
+      apply IHcstep2 with (c0 := c1); auto.
+    - apply impe2_exp_sound with (is_left := is_left) in H0; simpl in *.
+      apply Cstep_else with (e:=e) (c1:=c1) (c2:=c2); auto.
+      apply IHcstep2 with (c0 := c2); auto.
+    - apply impe2_exp_sound with (is_left := is_left) in H0; simpl in *.
+      destruct H1; apply l2_zero_or_one in H1; apply l2_zero_or_one in H6.
+        apply project_merge_inv_reg in H4; apply project_merge_inv_mem in H5;
+          destruct_conjs; unfold cleft in *; unfold cright in *; subst.
+        destruct is_left; [destruct H1 | destruct H6]; rewrite H in *.
+        1,3: apply Cstep_else with (e := e) (c1 := c1) (c2 := c2).
+        7,8: apply Cstep_if with (e := e) (c1 := c1) (c2 := c2).
+        all: auto; unfold_cfgs; simpl in *; try rewrite project_merge_inv_trace; auto.
+    - rewrite project_app_trace; simpl in *; subst.
+      apply Cstep_while_t with (e := e) (c := c)
+                                        (r := (project_reg r0 is_left))
+                                        (m := (project_mem m0 is_left)); auto.
+      now apply impe2_exp_sound with (is_left := is_left) in H0.
+      now apply IHcstep2_1 with (c0 := c).
+      (* XXX problem with inductive hypothesis *)
+      apply IHcstep2_2 with (c0 := (Cwhile e c)); auto.
+      admit.
+    - apply Cstep_while_f with (e := e) (c := c); auto.
+      now apply impe2_exp_sound with (is_left := is_left) in H0.
+    - apply impe2_exp_sound with (is_left := is_left) in H0; simpl in *;
+        apply project_merge_inv_reg in H4; apply project_merge_inv_mem in H5;
+          destruct_conjs; apply l2_zero_or_one in H1; apply l2_zero_or_one in H8;
+            unfold cleft in *; unfold cright in *.
+      destruct is_left; [destruct H1; rewrite H1 in * | destruct H8; rewrite H8 in *];
+        rewrite project_merge_inv_trace; subst; unfold_cfgs; simpl in *.
+      1,2: inversion H2; subst; try discriminate.
+      3,4: inversion H3; subst; try discriminate.
+      1,3: apply Cstep_while_f with (e := e) (c := c); auto.
+      all: apply Cstep_while_t with (e := e) (c := c) (r := r0) (m := m0); auto;
+        unfold_cfgs; simpl in *;
+          assert (c = hd) by congruence; rewrite H; auto;
+            assert ([Cwhile e c] = tl) by congruence; subst;
+              now apply -> cstep_seq_singleton in H10. 
+  Admitted.
+
+End Soundness.
+
+Section Completeness.
+  Lemma impe2_exp_complete : forall md d e r m v'i is_left,
+      estep md d (e, project_reg r is_left, project_mem m is_left) v'i ->
+      exists v', estep2 md d (e, r, m) v' /\ (project_value v' is_left = v'i).
+  Proof.
+    intros.
+    remember (e, project_reg r is_left, project_mem m is_left) as ecfg.
+    generalize dependent e.
+    induction H; intros; rewrite Heqecfg in H; simpl in *.
+    - exists (VSingle (Vnat n)); subst; split; auto; now constructor.
+    - exists (VSingle (Vloc l)); subst; split; auto; now constructor.
+    - exists (VSingle (Vlambda md c)); subst; split; auto; now constructor.
+    - exists (r x); split; auto. rewrite H. apply Estep2_var with (x:=x); auto.
+      rewrite Heqecfg in H0; simpl in *. rewrite <- H0.
+      now apply project_comm_reg.
+    - destruct IHestep1 with (e := e1). rewrite Heqecfg; auto.
+      destruct IHestep2 with (e := e2). rewrite Heqecfg; auto.
+      destruct_conjs.
+      exists (apply_op op x x0); split; auto.
+      apply Estep2_binop with (e1:=e1) (e2:=e2); auto.
+      split. now apply project_nat_contains_nat in H5.
+      now apply project_nat_contains_nat in H4.
+      apply project_value_apply_op; auto.
+    - assert (r0 = project_reg r is_left) by congruence.
+      assert (m0 = project_mem m is_left) by congruence.
+      destruct IHestep with (e0 := e). congruence.
+      destruct_conjs.
+      apply no_location_pairs in H6.
+      exists (m l); split.
+      apply Estep2_deref with (e := e) (r :=r) (m := m) (l := l); auto.
+      congruence.
+      rewrite <- H6; auto.
+      rewrite <- project_comm_mem; rewrite <- H4; auto.
+    Qed.
+      
+  Lemma impe2_complete : forall md d c r m r'1 m'1 t'1 r'2 m'2 t'2,
+      (cstep md d (project_ccfg (c, r, m) true) (r'1, m'1) t'1) /\
+      (cstep md d (project_ccfg (c, r, m) false) (r'2, m'2) t'2) ->
+      exists r' m' t',
+        cstep2 md d (c, r, m) (r', m') t' /\
+        (project_reg r' true) = r'1 /\
+        (project_mem m' true) = m'1 /\
+        (project_trace t' true) = t'1 /\
+        (project_reg r' false) = r'2 /\
+        (project_mem m' false) = m'2 /\
+        (project_trace t' false) = t'2.
+  Proof.
+    Local Ltac destruct_merge_inv :=
+      repeat
+        match goal with
+        | [ H : merge_mem _ _ _ |- _ ] => apply project_merge_inv_mem in H; destruct_conjs; auto
+        | [ H : merge_reg _ _ _ |- _ ] => apply project_merge_inv_reg in H; destruct_conjs; auto
+        | [ |- project_trace (merge_trace _) _ = _ ] => rewrite project_merge_inv_trace; auto
+        | _ => idtac
+        end.
+    
+    Local Ltac invert_cstep :=
+      match goal with
+      | [ H : cstep _ _ _ _ _ |- _ ] => inversion H; subst; try discriminate; simpl in *
+      end.
+
+    Local Ltac destruct_exp_complete :=
+      repeat
+        match goal with
+        | [ H : estep _ _ _ _ |- _ ] => apply impe2_exp_complete in H; destruct H; destruct_conjs
+        end.
+
+    Local Ltac e2_determinism x1 x2 H :=
+      assert (x1 = x2) by (apply estep2_deterministic with (v1 := x2) in H; auto); subst.
+
+    intros.
+    destruct H.
+    remember (project_ccfg (c, r, m) true) as ccfg1.
+    remember (r'1, m'1) as cterm1.
+    generalize dependent r'1; generalize dependent m'1.
+    generalize dependent r'2; generalize dependent m'2.
+    generalize dependent c; generalize dependent r; generalize dependent m.
+    revert t'2.
+    induction H; intros; unfold project_ccfg in *; rewrite Heqccfg1 in *; simpl in *;
+      invert_cstep; destruct_exp_complete.
+    (* SKIP *)
+    - do 3 eexists; repeat split; inversion Heqcterm1; subst; eauto.
+      econstructor; auto.
+      all: now cbn.
+    (* ASSIGN *)
+    - inversion H5; subst.
+      e2_determinism x1 x2 H.
+      do 3 eexists; repeat split; eauto.
+      eapply Cstep2_assign with (x := x0) (e := e0) (v := x2); eauto.
+      all: simpl; auto.
+      1,3: rewrite project_update_comm_reg; simpl; unfold project_ccfg; simpl.
+      all: congruence.
+    (* DECLASSIFY *)
+    - inversion H6; subst.
+      e2_determinism x1 x2 H.
+      do 3 eexists; repeat split; eauto.
+      eapply Cstep2_declassify with (x := x0) (v := x2); eauto.
+      all: simpl; auto.
+      1,3: rewrite project_update_comm_reg; simpl; unfold project_ccfg; simpl.
+      all: congruence.
+    (* UPDATE *)
+    - inversion H6; subst.
+      e2_determinism x x1 H; e2_determinism x0 x2 H4.
+      pose (no_location_pairs x1 l true H7).
+      do 3 eexists; repeat split; eauto.
+      eapply Cstep2_update; eauto.
+      all: simpl; auto.
+      rewrite <- e; unfold ccfg_to_ecfg2; auto.
+      congruence.
+      inversion Heqcterm1. apply project_update_comm_mem.
+      rewrite e in H2; simpl in H2; inversion H2.
+      apply project_update_comm_mem.
+    (* OUTPUT *)
+    - inversion H5; subst.
+      e2_determinism x x0 H.
+      do 3 eexists; repeat split; eauto.
+      eapply Cstep2_output with (e := e0); eauto.
+      all: simpl; auto; congruence.
+    (* CALL *)
+    - assert (e = e0) by congruence; rewrite H6 in *.
+      e2_determinism x x0 H.
+      destruct x0; subst.
+      + simpl in *. assert (c = c1) by congruence; subst.
+        edestruct IHcstep; unfold_cfgs; simpl; eauto. 
+        do 2 destruct H4; destruct_conjs.
+        exists x; exists x0; exists x1; repeat split.
+        apply Cstep2_call with (e := e0) (c := c1); auto.
+        unfold ccfg_to_ecfg2; simpl in *; subst; auto.
+        all: congruence.
+      + pose (merge_reg_exists r'1 r'2) as mr; destruct mr as [mr].
+        pose (merge_mem_exists m'1 m'2) as mm; destruct mm as [mm].
+        exists mr; exists mm; exists (merge_trace (tr, t'2)); repeat split.
+        eapply Cstep2_call_div; unfold_cfgs; simpl in *; subst; eauto.
+        1,2: inversion Heqcterm1; subst; auto.
+        all: destruct_merge_inv.
+    (* ENCLAVE *)
+    - inversion H9; subst.
+      edestruct IHcstep; eauto.
+      do 3 destruct H; destruct_conjs.
+      exists x; exists x0; exists x1; repeat split; auto.
+      eapply Cstep2_enclave; eauto.
+    (* SEQ_NIL *)
+    - exists r; exists m; exists []; repeat split.
+      apply Cstep2_seq_nil; auto.
+      all: inversion Heqcterm1; now subst.
+    (* SEQ_HD *)
+    - inversion H6; inversion Heqcterm1; subst; unfold_cfgs; simpl in *.
+      edestruct IHcstep1; eauto.
+      do 2 destruct H; destruct_conjs; subst.
+      edestruct IHcstep2; eauto.
+      do 2 destruct H2; destruct_conjs; subst.
+      do 3 eexists; repeat split; eauto.
+      eapply Cstep2_seq_hd; eauto.
+      all: rewrite project_app_trace; auto.
+    (* IF BOTH TRUE *)
+    - inversion H5; subst.
+      e2_determinism x x0 H.
+      destruct x0; subst.
+      + simpl in *; subst.
+        destruct IHcstep with (c := c0) (m'1 := m') (r'1 := r') (m'2 := m'2) (r'2 := r'2)
+                                        (t'2 := t'2) (m0 := m) (r0 := r); auto.
+        do 3 destruct H4; destruct_conjs.
+        exists x; exists x0; exists x1; repeat split; auto.
+        apply Cstep2_if with (e := e0) (c1 := c0) (c2 := c3); auto.
+        all: inversion Heqcterm1; subst; auto.
+      + pose (merge_reg_exists r'1 r'2) as mr; destruct mr as [mr].
+        pose (merge_mem_exists m'1 m'2) as mm; destruct mm as [mm].
+        exists mr; exists mm; exists (merge_trace (tr, t'2)); repeat split.
+        apply Cstep2_if_div with (e := e0) (c1 := c0) (c2 := c3) (n1 := 1) (n2 := 1)
+                                           (r1 := r') (m1 := m') (r2 := r'2) (m2 := m'2); auto.
+        unfold_cfgs; simpl in *; now subst.
+        all: inversion Heqcterm1; subst; auto; destruct_merge_inv.
+    (* IF TRUE, FALSE *)
+    - inversion H5; subst.
+      e2_determinism x x0 H.
+      destruct x0; subst.
+      + simpl in *; subst; discriminate.
+      + pose (merge_reg_exists r'1 r'2) as mr; destruct mr as [mr].
+        pose (merge_mem_exists m'1 m'2) as mm; destruct mm as [mm].
+        exists mr; exists mm; exists (merge_trace (tr, t'2)); repeat split.
+        apply Cstep2_if_div with (e := e0) (c1 := c0) (c2 := c3) (n1 := 1) (n2 := 0)
+                                           (r1 := r') (m1 := m') (r2 := r'2) (m2 := m'2); auto.
+        unfold_cfgs; simpl in *; now subst.
+        all: inversion Heqcterm1; subst; auto; destruct_merge_inv.
+    (* IF FALSE, TRUE *)
+    - inversion H5; subst.
+      e2_determinism x x0 H.
+      destruct x0; subst.
+      + simpl in *; subst; discriminate.
+      + pose (merge_reg_exists r'1 r'2) as mr; destruct mr as [mr].
+        pose (merge_mem_exists m'1 m'2) as mm; destruct mm as [mm].
+        exists mr; exists mm; exists (merge_trace (tr, t'2)); repeat split.
+        apply Cstep2_if_div with (e := e0) (c1 := c0) (c2 := c3) (n1 := 0) (n2 := 1)
+                                           (r1 := r') (m1 := m') (r2 := r'2) (m2 := m'2); auto.
+        unfold_cfgs; simpl in *; now subst.
+        all: inversion Heqcterm1; subst; auto; destruct_merge_inv.    
+    - inversion H5; subst.
+      e2_determinism x x0 H.
+      destruct x0; subst.
+      + simpl in *; subst.
+        destruct IHcstep with (c := c3) (m'1 := m') (r'1 := r') (m'2 := m'2) (r'2 := r'2)
+                                        (t'2 := t'2) (m0 := m) (r0 := r); auto.
+        do 3 destruct H4; destruct_conjs.
+        exists x; exists x0; exists x1; repeat split; auto.
+        apply Cstep2_else with (e := e0) (c1 := c0) (c2 := c3); auto.
+        all: inversion Heqcterm1; subst; auto.
+      + pose (merge_reg_exists r'1 r'2) as mr; destruct mr as [mr].
+        pose (merge_mem_exists m'1 m'2) as mm; destruct mm as [mm].
+        exists mr; exists mm; exists (merge_trace (tr, t'2)); repeat split.
+        apply Cstep2_if_div with (e := e0) (c1 := c0) (c2 := c3) (n1 := 0) (n2 := 0)
+                                           (r1 := r') (m1 := m') (r2 := r'2) (m2 := m'2); auto.
+        unfold_cfgs; simpl in *; now subst.
+        all: inversion Heqcterm1; subst; auto; destruct_merge_inv.
+    (* WHILE BOTH TRUE *)
+    - inversion H6; subst.
+      e2_determinism x x0 H.
+      destruct x0; subst.
+      + admit.
+      + pose (merge_reg_exists r'1 r'2) as mr; destruct mr as [mr].
+        pose (merge_mem_exists m'1 m'2) as mm; destruct mm as [mm].
+        exists mr; exists mm; exists (merge_trace (tr ++ tr', tr0 ++ tr'0)); repeat split.
+        eapply Cstep2_while_div; eauto.
+        all: unfold_cfgs; simpl in *; inversion Heqcterm1; subst; auto.
+        1,2: eapply Cstep_seq_hd; simpl; eauto; apply cstep_seq_singleton; auto.
+        all: destruct_merge_inv.
+    (* WHILE TRUE, FALSE *)
+    - inversion H9; subst.
+      e2_determinism x x0 H.
+      destruct x0; subst.
+      + simpl in *; subst; discriminate.
+      + admit.
+    (* WHILE FALSE, TRUE *)
+    - inversion H4; subst.
+      e2_determinism x x0 H.
+      destruct x0; subst.
+      + simpl in *; subst; discriminate.
+      + admit.
+    (* WHILE BOTH FALSE *)
+    - admit.
+  Admitted.
+  
+End Completeness.
