ImpE2Helpers.v
@@ -1,0 +1,642 @@
+Require Import Bool Arith List Omega ListSet.
+Require Import Recdef Morphisms.
+Require Import Program.Tactics.
+Require Import Relation_Operators.
+Require FMapList.
+Require FMapFacts.
+Require Import Classical.
+Require Import Coq.Classes.RelationClasses.
+Require Import OrderedType OrderedTypeEx DecidableType.
+Require Import Coq.Logic.FunctionalExtensionality.
+Require Import Sorting.Permutation.
+Require Import Coq.Sets.Ensembles.
+Import ListNotations.
+Require Import Common.
+Require Import ImpE.
+Require Import ImpE2.
+
+Ltac unfold_cfgs :=
+  unfold ccfg_update_reg2 in *;
+  unfold ccfg_to_ecfg2 in *;
+  unfold ccfg_reg in *;
+  unfold ccfg_mem in *;
+  unfold ccfg_com in *;
+  unfold ccfg_reg2 in *;
+  unfold ccfg_mem2 in *;
+  unfold ccfg_com2 in *;
+  unfold ecfg_exp2 in *;
+  unfold ecfg_reg2 in *;
+  unfold ecfg_update_exp2 in *;
+  unfold ccfg_update_com2 in *;
+  unfold ccfg_update_mem2 in *;
+  unfold ccfg_update_mem in *;
+  unfold ccfg_update_reg in *;
+  unfold ccfg_update_com in *;
+  unfold ccfg_to_ecfg in *;
+  unfold project_ccfg.
+
+Section Misc.
+  Axiom No_Pointers2 : forall (m: mem2) l,
+    (forall l', m l <> VSingle (Vloc l')) /\
+    (forall l' l'', m l <> VPair (Vloc l') (Vloc l'')).
+  
+  Lemma l2_zero_or_one (n : nat) : n < 2 -> n = 0 \/ n = 1.
+  Proof. omega. Qed.
+
+  Lemma filter_app (f:event -> bool) l1 l2:
+    filter f (l1 ++ l2) = filter f l1 ++ filter f l2.
+  Proof.
+    induction l1; simpl; auto. rewrite IHl1. destruct (f a); auto.
+  Qed.
+End Misc.
+
+Section Project_Merge.
+  (* XXX: these assumptions are gross, but the semantics become a mess if we
+     dont' have them... *)
+
+  Lemma project_nat_contains_nat : forall v n is_left,
+      project_value v is_left = Vnat n ->
+      contains_nat v.
+  Proof.
+  Admitted.
+
+  Lemma no_location_pairs : forall v l is_left,
+      project_value v is_left = Vloc l ->
+      v = VSingle (Vloc l).
+  Proof.
+  Admitted.
+  
+  Lemma project_comm_reg : forall r b x,
+      (project_reg r b) x = project_value (r x) b.
+  Proof.
+    intros; unfold project_reg; destruct (r x); auto.
+  Qed.
+
+  Lemma project_comm_mem : forall m b x,
+      (project_mem m b) x = project_value (m x) b.
+  Proof.
+    intros; unfold project_mem; destruct (m x); auto.
+  Qed.
+
+  (* XXX: this might be a pain to prove with registers as functions. Used below in soundness. *)
+  Lemma project_update_comm_reg : forall ccfg x v is_left,
+      project_reg (ccfg_update_reg2 ccfg x v) is_left = 
+      ccfg_update_reg (project_ccfg ccfg is_left) x (project_value v is_left).
+  Proof.
+    intros.
+    extensionality z.
+    unfold project_reg; unfold ccfg_update_reg; unfold ccfg_update_reg2.
+    destruct (z =? x).
+    - unfold project_value; auto.
+    - simpl; now unfold project_reg.
+  Qed.
+
+  Lemma project_update_comm_mem : forall ccfg l v is_left,
+      project_mem (ccfg_update_mem2 ccfg l v) is_left = 
+      ccfg_update_mem (project_ccfg ccfg is_left) l (project_value v is_left).
+  Proof.
+    intros.
+    extensionality z.
+    unfold_cfgs; unfold ccfg_update_mem2; unfold project_mem.
+    destruct (z =? l).
+    - unfold project_value; auto.
+    - simpl; now unfold project_mem.
+  Qed.
+
+  (* XXX: these lemmata are necessary because merge_reg and merge_mem are propositional *)
+  Lemma merge_reg_exists : forall r1 r2,
+      exists r, merge_reg r1 r2 r.
+  Proof.
+  Admitted.
+
+  Lemma merge_mem_exists : forall m1 m2,
+      exists m, merge_mem m1 m2 m.
+  Proof.
+  Admitted.
+  
+  Lemma project_merge_inv_reg : forall r1 r2 r,
+      merge_reg r1 r2 r -> (project_reg r true = r1) /\ (project_reg r false = r2).
+  Proof.
+  Admitted.
+
+  Lemma project_merge_inv_mem : forall m1 m2 m,
+      merge_mem m1 m2 m <-> (project_mem m true = m1) /\ (project_mem m false = m2).
+  Proof.
+  Admitted.
+
+  Lemma project_merge_inv_trace : forall t1 t2 is_left,
+      project_trace (merge_trace (t1, t2)) is_left = (if is_left then t1 else t2).
+  Proof.
+  Admitted.
+
+  Lemma project_app_trace : forall t1 t2 is_left,
+      project_trace (t1 ++ t2) is_left =
+      (project_trace t1 is_left) ++ (project_trace t2 is_left).
+  Proof.
+    intros.
+    induction t1.
+    - rewrite app_nil_l; now cbn.
+    - cbn; rewrite IHt1; now destruct (event2_to_event a is_left).
+  Qed.
+
+  Lemma contains_nat_project_nat : forall v is_left,
+      contains_nat v -> exists n, project_value v is_left = Vnat n.
+  Proof.
+    intros.
+    destruct v.
+    - unfold contains_nat in H; destruct H.
+      + destruct H; exists x; simpl; congruence.
+      + destruct H; destruct H; discriminate.
+    - unfold contains_nat in H; destruct H.
+      + destruct H; discriminate.
+      + destruct H; destruct H.
+        destruct is_left; [exists x | exists x0]; simpl; congruence.
+  Qed.
+
+  Lemma project_value_apply_op : forall op v1 v2 n1 n2 is_left,
+      project_value v1 is_left = Vnat n1 ->
+      project_value v2 is_left = Vnat n2 ->
+      (project_value (apply_op op v1 v2) is_left) = Vnat (op n1 n2).
+  Proof.
+  Admitted.
+
+End Project_Merge.
+
+Section Semantics.
+  (* XXX: thought I needed this for exp_output_wf, didn't use it. Might still be useful...? *)
+  Lemma estep2_deterministic : forall md d e r m v1 v2,
+      estep2 md d (e, r, m) v1 ->
+      estep2 md d (e, r, m) v2 ->
+      v1 = v2.
+  Proof.
+    intros; revert H0; revert v2.
+    induction H; intros; destruct ecfg as [[e' r'] m']; simpl in *; try rewrite H in H0.
+    1-3: inversion H0; subst; try discriminate; simpl in H1; congruence.
+    inversion H1; subst; try discriminate; simpl in *; congruence.
+    - rewrite H in H3; inversion H3; try discriminate; simpl in *;
+        assert (e1 = e0) by congruence; assert (e2 = e3) by congruence;
+          subst; apply IHestep2_1 in H5; apply IHestep2_2 in H6; congruence.
+   - rewrite H in H3; inversion H3; subst; try discriminate; simpl in *.
+      assert (e0 = e1) by congruence.
+      assert (r0 = r1) by congruence.
+      assert (m0 = m1) by congruence.
+      subst. apply IHestep2 in H5. assert (l = l0) by congruence; now subst.
+  Qed.  
+ 
+  (* Executing a singleton sequence is the same as executing the command *)
+  Lemma cstep_seq_singleton : forall md d c r m r' m' t,
+      cstep md d (Cseq [c], r, m) (r', m') t <->
+      cstep md d (c, r, m) (r', m') t.
+    split; intros.
+    - inversion H; subst; try discriminate; unfold_cfgs.
+      simpl in H3.
+      simpl in H2; assert (tl = []) by congruence.
+      rewrite H0 in H7. inversion H7; subst; try discriminate.
+      rewrite app_nil_r; congruence.
+    - eapply Cstep_seq_hd; simpl; eauto.
+      try econstructor; now simpl.
+      now rewrite app_nil_r.
+  Qed.
+   Lemma apply_op_pair (op : nat -> nat -> nat) (v1 v2: val2) :
+       contains_nat v1 /\ contains_nat v2 /\
+       (exists v3 v4, apply_op op v1 v2 = VPair v3 v4) <->
+       exists v' v'', contains_nat v1 /\ contains_nat v2 /\
+                      (v1 = VPair v' v'' \/ v2 = VPair v' v'').
+   Proof.
+     intros.
+     split; intros; destruct_pairs.
+     induction v1, v2; unfold apply_op in *; destruct H1; destruct H1.
+     destruct v, v0; try discriminate.
+     - destruct v, v0; try discriminate.
+       destruct v1; try discriminate.
+       exists (Vnat n0). exists (Vnat n1).
+       split; auto. 
+     - destruct v, v0; try discriminate.
+       1-4: unfold contains_nat in H; destruct H; destruct H;
+         [discriminate | destruct H; inversion H].
+       2-5: unfold contains_nat in H; destruct H; destruct H;
+         [discriminate | destruct H; inversion H].
+       exists (Vnat n). exists (Vnat n0). split; auto.
+     - destruct v, v0; try discriminate.
+       1-4: unfold contains_nat in H; destruct H; destruct H;
+         [discriminate | destruct H; inversion H].
+       2-5: unfold contains_nat in H; destruct H; destruct H;
+         [discriminate | destruct H; inversion H].
+       exists (Vnat n). exists (Vnat n0). split; auto.
+     - destruct H. destruct H. destruct H; destruct_pairs.
+       split; [ | split]; auto.
+       destruct H1.
+       -- rewrite H1. destruct v2; destruct v.
+          destruct H0; destruct H0; [discriminate | destruct H0; inversion H0].
+          2-5: destruct H0; destruct H0; [discriminate | destruct H0; inversion H0].
+          unfold apply_op.
+          exists x. exists x0. destruct x; auto. destruct x0; auto.
+          unfold apply_op.
+          destruct x; auto. exists (Vlambda m c). exists x0; auto.
+          destruct x0; auto. exists (Vnat n0). exists (Vlambda m c); auto.
+          exists (Vnat (op n0 x1)). exists (Vnat (op n1 x2)); auto.
+          exists (Vnat n0). exists (Vloc l). auto.
+          exists (Vloc l). exists x0. auto.
+       -- rewrite H1 in *. destruct v1; destruct v.
+          destruct H; destruct H; [discriminate | destruct H; inversion H].
+          2-5: destruct H; destruct H; [discriminate | destruct H; inversion H].
+          unfold apply_op.
+          destruct x. destruct H0; destruct H0; [discriminate | destruct H0; inversion H0].
+          destruct x0. destruct H0; destruct H0; [discriminate | destruct H0; inversion H0].
+          exists (Vnat (op n n0)). exists (Vnat (op n n1)). auto.
+          destruct H0; destruct H0; [discriminate | destruct H0; inversion H0].
+          destruct H0; destruct H0; [discriminate | destruct H0; inversion H0].
+          unfold apply_op.
+          destruct x; auto. exists (Vnat x1). exists (Vnat x2). auto.
+          destruct x0; auto. exists (Vnat x1). exists (Vnat x2); auto.
+          exists (Vnat (op x1 n0)). exists (Vnat (op x2 n1)); auto.
+          1-2: exists (Vnat x1); exists (Vnat x2); auto.
+   Qed.
+End Semantics.
+
+Section Typing.
+  (* XXX prove type preservation *)
+  (* XXX I feel like this should be provable from something... but our typing *)
+  (* system seems to be lacking something *)
+  Lemma call_fxn_typ : forall pc md G d e r m Gm p Gp q c Gout,
+    com_type pc md G d (Ccall e) Gout ->
+    estep md d (e,r,m) (Vlambda md c) ->
+    exp_type md G d e (Typ (Tlambda Gm p md Gp) q) <-> com_type p md Gm d c Gp.
+  Proof.
+    intros.
+    inversion H0; try discriminate; subst.
+  Admitted.
+
+  (* XXX nothing connecting loc_context to actual type at location *)
+  Lemma ref_type : forall pc md md' d e1 e2 r m G bt s p0 p p' q l rt,
+    com_type pc md G d (Cupdate e1 e2) G ->
+    estep2 md d (e1, r, m) (VSingle (Vloc l)) ->
+    exp_type md G d e1 (Typ (Tref (Typ s p) md' Mut) q) ->
+    exp_type md G d e2 (Typ s p') ->
+    Loc_Contxt l = Some (Typ bt p0, rt) ->
+    s = bt /\ p = p0.
+  Proof.
+  Admitted.
+  
+  Lemma subsumption : forall pc1 pc2 md d G1 G1' G2 G2' c,
+      com_type pc1 md G1 d c G1' ->
+      sec_level_le pc2 pc1 ->
+      context_le G2 G1 ->
+      context_le G1' G2' ->
+      (* XXX not including well-typed contexts *)
+      com_type pc2 md G2 d c G2'.
+  Admitted.
+End Typing.
+
+(*******************************************************************************
+*
+* SECURITY HELPER LEMMAS
+*
+*******************************************************************************)
+
+Section Security.
+  Lemma tobs_sec_level_app (sl: sec_level) (l l': trace) :
+    tobs_sec_level sl l ++ tobs_sec_level sl l' = tobs_sec_level sl (l ++ l').
+  Proof.
+    unfold tobs_sec_level. now rewrite (filter_app _ l l').
+  Qed.
+
+  (* XXX assume that if the value is a location, then the policy on the location *)
+  (* is protected by S. This should be fine because we're assuming this for *)
+  (* memories that are indistinguishable *)
+  Lemma econfig2_locs_protected (e: exp):
+    forall G d r m v v1 v2 bt bt' p p' q md md' rt e',
+      mem_sl_ind L ->
+      v = VPair v1 v2 ->
+      exp_type md G d e (Typ bt p) ->
+      estep2 md d (e,r,m) v ->
+      e = Ederef e' ->
+      exp_type md G d e' (Typ (Tref (Typ bt' p') md' rt) q) ->
+      protected q.
+  Proof.
+  Admitted.
+
+  Lemma econfig2_pair_protected : forall md G d e p r m v v1 v2 bt,
+      v = VPair v1 v2 ->
+      exp_type md G d e (Typ bt p) ->
+      estep2 md d (e,r,m) v ->
+      cterm2_ok G d r m ->
+      protected p.
+  Proof.
+    intros.
+    remember (e,r,m) as ecfg.
+    generalize dependent e.
+    generalize dependent v1.
+    generalize dependent v2.
+    generalize dependent p.
+    pose H1 as Hestep2.
+    induction Hestep2; intros; subst; try discriminate; unfold_cfgs;
+      unfold cterm2_ok in *; destruct_pairs; subst.
+     - inversion H4; subst.
+       apply (H0 x v1 v2 bt p); split; auto.
+     - rewrite H3 in *.
+       assert (exists v' v'', v1 = VPair v' v'' \/ v2 = VPair v' v'').
+       pose (apply_op_pair op v1 v2) as Hop_pair.
+       destruct Hop_pair as [Hop1 Hop2].
+       assert (contains_nat v1 /\ contains_nat v2 /\
+               (exists v3 v4 : val, apply_op op v1 v2 = VPair v3 v4)).
+       split; auto. split; auto. exists v3. exists v0.  auto.
+       apply Hop1 in H. destruct H. destruct H. destruct_pairs.
+       exists x. exists x0. auto.
+       inversion H4; subst; try discriminate.
+       destruct H. destruct H; destruct H.
+       -- assert (protected p0).
+          eapply (IHHestep2_1 Hestep2_1). unfold cterm2_ok; auto.
+          apply H. apply H14. auto.
+          now apply (join_protected_l p0 q).
+       -- assert (protected q ).
+          eapply (IHHestep2_2 Hestep2_2). unfold cterm2_ok; auto.
+          apply H. apply H18. auto.
+          now apply (join_protected_r p0 q).
+     - inversion Heqecfg; subst.
+       inversion H5; subst.
+       assert (protected q).
+       apply (econfig2_locs_protected (Ederef e) G d r m (m l) v1 v2 bt bt
+                                      (sec_level_join p0 q) p0 q md md' rt e); auto.
+       apply (join_protected_r p0 q); auto.
+  Qed.
+  
+  Lemma protected_typ_no_obs_output r2 m2 is_left : forall pc md d G c G' r' m' tr,
+    com_type pc md G d c G' ->
+    protected pc ->
+    cstep md d (c,project_reg r2 is_left,project_mem m2 is_left) (r',m') tr ->
+    tobs_sec_level L tr = [].
+  Proof.
+    intros. remember (c,project_reg r2 is_left,project_mem m2 is_left) as ccfg.
+    generalize dependent pc. generalize dependent G. generalize dependent G'.
+    generalize dependent c. generalize dependent r2. generalize dependent m2.
+    induction H1; intros; inversion H; subst; auto;
+      unfold_cfgs; unfold_cfgs; unfold_cfgs; subst.
+    - inversion H2; try discriminate; subst.
+      rewrite join_protected_r in H12; auto.
+      unfold sec_level_le in H12; destruct sl; intuition.
+    - inversion H2; try discriminate; subst.
+      assert (com_type p md Gm d c Gp).
+      eapply call_fxn_typ; eauto. 
+      eapply (IHcstep m2 r2 c); eauto. 
+      rewrite join_protected_l in H6; auto.
+      unfold sec_level_le in H6; destruct p; intuition. unfold protected; auto.
+    - inversion H2; try discriminate; subst.
+      inversion H; subst.
+      eapply (IHcstep m2 r2 c'); eauto.
+    - inversion H1; try discriminate; subst.
+      assert (tobs_sec_level L tr = []).
+      eapply (IHcstep1 m2 r2 hd); eauto.
+      assert (tobs_sec_level L tr' = []).
+      pose (merge_reg_exists r r). destruct e.
+      pose (merge_mem_exists m m). destruct e.
+      eapply (IHcstep2 x0 x (Cseq tl)); eauto.
+      apply project_merge_inv_mem in H3. apply project_merge_inv_reg in H0. destruct_pairs.
+      destruct is_left. rewrite H0, H3; auto. rewrite H5, H6; auto.
+      rewrite <- tobs_sec_level_app. rewrite H; rewrite H0; auto.
+    - inversion H2; try discriminate; subst.
+      eapply (IHcstep m2 r2 c1); eauto.
+      rewrite join_protected_l in H15; auto.
+      unfold sec_level_le in H15; destruct pc'; intuition; now unfold protected.
+    - inversion H2; try discriminate; subst.
+      eapply (IHcstep m2 r2 c2); eauto.
+      rewrite join_protected_l in H15; auto.
+      unfold sec_level_le in H15; destruct pc'; intuition; now unfold protected.
+    - inversion H1; try discriminate; subst.
+      assert (tobs_sec_level L tr = []).
+      eapply (IHcstep1 m2 r2 c); eauto.
+      rewrite join_protected_l in H11; auto.
+      unfold sec_level_le in H11; destruct pc'; intuition; now unfold protected.
+      assert (tobs_sec_level L tr' = []).
+      pose (merge_reg_exists r r). destruct e0.
+      pose (merge_mem_exists m m). destruct e0.
+      eapply (IHcstep2 x0 x (Cwhile e c)); eauto.
+      apply project_merge_inv_reg in H3. apply project_merge_inv_mem in H7. destruct_pairs.
+      destruct is_left. rewrite H7, H3; auto. rewrite H8, H9; auto.
+      rewrite <- tobs_sec_level_app. rewrite H; rewrite H3; auto.
+  Qed.
+
+  Lemma protected_c_in_while_no_obs_output : forall pc pc' md d G e c r m r' m' tr,
+    com_type pc md G d (Cwhile e c) G ->
+    com_type pc' md G d c G ->
+    protected pc' ->
+    cstep md d (Cwhile e c, r, m) (r',m') tr ->
+    tobs_sec_level L tr = [].
+  Proof.
+    intros. inversion H; try discriminate; subst.
+  Admitted.
+    
+  Lemma protected_while_no_obs_output : forall pc pc' md d G e c r m r' m' tr,
+      com_type pc md G d (Cwhile e c) G ->
+      com_type pc' md G d c G ->
+      protected pc' ->
+      cstep md d (Cseq [c; Cwhile e c],r,m) (r',m') tr ->
+      tobs_sec_level L tr = [].
+  Proof.
+    intros.
+    inversion H2; try discriminate; subst; unfold_cfgs; unfold_cfgs.
+    inversion H5; subst.
+    assert (tobs_sec_level L tr0 = []).
+    pose (merge_reg_exists r r). pose (merge_mem_exists m m).
+    destruct e0, e1.
+    apply project_merge_inv_reg in H3; apply project_merge_inv_mem in H4; destruct_pairs.
+    assert (cstep md d (hd, project_reg x true, project_mem x0 true) (r0, m0) tr0).
+    rewrite H4, H3; auto.
+    pose (protected_typ_no_obs_output x x0 true pc' md d G hd G r0 m0 tr0); auto.
+    assert (tobs_sec_level L tr' = []).
+    rewrite cstep_seq_singleton in H10.
+    eapply protected_c_in_while_no_obs_output; eauto.
+    now rewrite <- tobs_sec_level_app, H3, H4.
+  Qed.
+
+  Lemma diff_loc_protected : forall l,
+      mem_sl_ind L ->
+      (project_mem minit true) l <> (project_mem minit false) l ->
+      protected (g0 l).
+  Proof.
+    intros. remember (g0 l) as p.
+    unfold mem_sl_ind in *.
+    rewrite <- (H l) in H0. unfold sec_level_le in H0. 
+    destruct p; rewrite <- Heqp in H0. intuition.
+    now unfold protected.
+  Qed.
+  
+  Lemma vpair_if_diff : forall m1 m2 v1 v2 l,
+      merge_mem m1 m2 minit ->
+      minit l = VPair v1 v2 -> m1 l <> m2 l.
+  Proof.
+    intros. inversion H; subst. apply (H1 l) in H0; destruct_pairs; auto.
+  Qed.
+
+  (* We somehow need to know that if c performs an assignment or update of x, then *)
+  (* the type of x in the env is at a higher security level than pc' *)
+  (* Otherwise, the reg/mem and context does not change *)
+  Definition assign_in (c: com) (x: var) : Prop.
+  Admitted.
+  (*
+    match c with
+    | Cassign x _ => True
+    | Ccall e => assign_in_exp e x
+    | Cenclave _ c' => assign_in c' x
+    | Cseq ls => List.fold_left (fun b c' => b /\ (assign_in c' x)) ls False
+    | Cif e c1 c2 => assign_in c1 x \/ assign_in c2 x
+    | Cwhile e c => assign_in c x 
+    | _ => False
+    end
+  with assign_in_exp e x : Prop :=
+         forall md d r m c1 c2 c',
+           (estep2 md d (Ederef e,r,m) (VPair (Vlambda md c1) (Vlambda md c2))
+            /\ assign_in c1 x /\ assign_in c2 x)
+           \/ (estep2 md d (e,r,m) (VSingle (Vlambda md c')) /\ assign_in c' x).
+   *)
+  Lemma assign_not_in_call_div : forall e x md d r m c1 c2,
+      ~assign_in (Ccall e) x <-> 
+      (estep2 md d (e,r,m) (VPair (Vlambda md c1) (Vlambda md c2)))
+      /\ (~assign_in c1 x /\ ~assign_in c2 x).
+  Admitted.
+  Lemma assign_in_if_else : forall e c1 c2 x,
+      assign_in (Cif e c1 c2) x <-> assign_in c1 x \/ assign_in c2 x.
+  Admitted.
+  Lemma assign_in_while : forall e c x,
+      assign_in (Cwhile e c) x <-> assign_in c x.
+  Admitted.
+  Lemma assign_in_dec : forall c x, {assign_in c x} + {~assign_in c x}.
+  Proof.
+  Admitted.
+
+  Lemma assignment_more_secure : forall pc md d c G G' x bt q,
+    com_type pc md G d c G' ->
+    assign_in c x ->
+    G' x = Some (Typ bt q) ->
+    sec_level_le pc q.
+  Proof.
+  Admitted.
+  Lemma no_assign_reg_context_constant : forall md d c r m r' m' tr x pc G G',
+      cstep2 md d (c, r, m) (r', m') tr ->
+      com_type pc md G d c G' ->
+      ~assign_in c x ->
+      r x = r' x /\ G x = G' x.
+  Proof.
+  Admitted.
+
+  (* Same thing as assignments for updates *)
+  Definition update_in (c: com) (l: location) : Prop.
+  Admitted. (*
+    match c with
+    | Cupdate e1 e2 => forall l',
+        estep2 md d (e1, r, m) (VSingle (Vloc l))
+        \/ estep2 md d (e1, r, m) (VPair (Vloc l), (Vloc l'))
+        \/ estep2 md d (e1, r, m) (VPair (Vloc l'), (Vloc l))
+    | Ccall (Elambda _ c') => update_in c' l
+    | Ccall e => estep2 md d (e,r,m) (VPair (Vlambda md c1) (Vlambda md c2)) ->
+                 update_in c1 /\ update_in c2.
+    | Ccall e => estep2 md d (e,r,m) (VSingle (Vlambda md c')) ->
+                 update_in c'.
+    | Cenclave _ c' => update_in c' l
+    | Cseq ls => List.fold_left (fun b c' => b /\ (update_in c' l)) ls False
+    | Cif e c1 c2 => update_in c1 l \/ update_in c2 l
+    | Cwhile e c => update_in c l
+    | _ => False
+    end.*)
+  Lemma update_not_in_call_div : forall e x md d r m c1 c2,
+      ~update_in (Ccall e) x <-> 
+      (estep2 md d (e,r,m) (VPair (Vlambda md c1) (Vlambda md c2)))
+      /\ (~update_in c1 x /\ ~update_in c2 x).
+  Admitted.
+  Lemma update_in_if_else : forall e c1 c2 x,
+      update_in (Cif e c1 c2) x <-> update_in c1 x \/ update_in c2 x.
+  Admitted.
+  Lemma update_in_while : forall e c x,
+      update_in (Cwhile e c) x <-> update_in c x.
+  Admitted.
+  Lemma update_in_dec : forall c l, {update_in c l} + {~update_in c l}.
+  Admitted.
+  Lemma update_more_secure : forall pc md d c G G' x bt q rt,
+    com_type pc md G d c G' ->
+    update_in c x ->
+    Loc_Contxt x = Some (Typ bt q, rt) ->
+    sec_level_le pc q.
+  Proof.
+  Admitted.
+  Lemma no_update_mem_constant : forall md d c r m r' m' tr x pc G G',
+      cstep2 md d (c, r, m) (r', m') tr ->
+      com_type pc md G d c G' ->
+      ~update_in c x ->
+      m x = m' x.
+  Proof.
+  Admitted.
+
+  Lemma loc_in_exp_deref : forall e md G d typ r m l,
+      is_escape_hatch e ->
+      exp_type md G d (Ederef e) typ ->
+      estep2 md d (e,r,m) (VSingle (Vloc l)) ->
+      loc_in_exp e l.
+  Proof.
+    intros. remember (e, r, m) as ecfg.
+    generalize dependent e. generalize dependent r. generalize dependent m.
+    generalize dependent l. generalize dependent typ.
+    unfold is_escape_hatch in *; destruct_pairs.
+    induction e; intros; unfold_cfgs; subst; unfold loc_in_exp; auto;
+      inversion Heqecfg; subst.
+    -- inversion H1; try discriminate.
+    -- unfold exp_novars in H; simpl in *. omega.
+    -- inversion H0; try discriminate; subst.
+       inversion H3.
+    -- inversion H1; try discriminate; subst; unfold_cfgs.
+       now inversion H6.
+    -- inversion H1; try discriminate; subst; unfold_cfgs. inversion H2; subst.
+       pose (No_Pointers2 m l0); destruct_pairs.
+       pose (H6 l). intuition. apply n in H4. omega.
+    -- inversion H0; try discriminate; subst.
+       inversion H3.
+  Qed.
+  
+  Lemma same_mem_locs_evals_same_value : forall e r m md d G typ vfin,
+      exp_type md G d e typ ->
+      estep2 md d (e,r,m) vfin ->
+      is_escape_hatch e ->      (forall l, loc_in_exp e l -> exists v, m l = VSingle v) ->
+      exists v, vfin = (VSingle v).
+  Proof.
+    intros e r m md d G typ vfin Hwt Hestep Heh Helocs. unfold is_escape_hatch in *; destruct_pairs.
+    generalize dependent typ. generalize dependent vfin.
+    induction e; intros; inversion Hestep; try discriminate; unfold_cfgs. subst.
+    - exists (Vnat n0); auto.
+    - unfold exp_novars in *; simpl in *; omega.
+    - inversion H1; subst.
+      inversion Hwt; try discriminate; subst.
+
+      assert (exp_novars e0 /\ exp_novars e3).
+      unfold exp_novars in *. now inversion H.
+
+      assert (exp_locs_immutable e0 /\ exp_locs_immutable e3).
+      inversion H0. unfold exp_locs_immutable in *; auto.
+
+      assert (forall l : location, loc_in_exp e0 l -> exists v, m l = VSingle v).
+      intros. pose (Helocs l) as nolocs. unfold loc_in_exp in nolocs. destruct nolocs.
+      left; auto.
+      exists x. destruct H3; auto.
+      assert (forall l : location, loc_in_exp e3 l -> exists v, m l = VSingle v).
+      intros. pose (Helocs l) as nolocs. unfold loc_in_exp in nolocs. destruct nolocs.
+      right; auto.
+      exists x. destruct H3; auto. 
+      destruct_pairs.
+      
+      pose (IHe1 H5 H6 H7 _ H2 _ H12) as He1; destruct He1 as [x He1].
+      pose (IHe2 H10 H9 H8 _ H3 _ H13) as He2; destruct He2 as [y He2].
+      unfold contains_nat in *.
+      destruct H4 as [[n0 H41']|[n0 [n1 blah]]]; destruct H11 as [[n4 H11']|[n2 [n3 blah']]];
+        subst; try discriminate.
+      exists (Vnat (op n0 n4)). now unfold apply_op.
+    - exists (Vloc l0); auto.
+    - inversion H1; subst. 
+      assert (loc_in_exp e0 l).
+      eapply loc_in_exp_deref; eauto.
+      unfold is_escape_hatch. split; [inversion H | inversion H0]; auto.
+      assert (loc_in_exp (Ederef e0) l).
+      unfold loc_in_exp in *; auto.
+      destruct (Helocs l H5). exists x. auto. 
+    - subst. exists (Vlambda md c0); auto.
+  Qed.
+End Security.
+
+     
