ImpE2Security.v
@@ -1,0 +1,670 @@
+Require Import Bool Arith List Omega ListSet.
+Require Import Recdef Morphisms.
+Require Import Program.Tactics.
+Require Import Relation_Operators.
+Require FMapList.
+Require FMapFacts.
+Require Import Classical.
+Require Import Coq.Classes.RelationClasses.
+Require Import OrderedType OrderedTypeEx DecidableType.
+Require Import Coq.Logic.FunctionalExtensionality.
+Require Import Sorting.Permutation.
+Require Import Coq.Sets.Ensembles.
+Import ListNotations.
+Require Import Common.
+Require Import ImpE.
+Require Import ImpE2.
+Require Import ImpE2Helpers.
+Require Import ImpE2Adequacy.
+
+Ltac unfold_cfgs :=
+  unfold ccfg_update_reg2 in *;
+  unfold ccfg_to_ecfg2 in *;
+  unfold ccfg_reg in *;
+  unfold ccfg_mem in *;
+  unfold ccfg_com in *;
+  unfold ccfg_reg2 in *;
+  unfold ccfg_mem2 in *;
+  unfold ccfg_com2 in *;
+  unfold ecfg_exp2 in *;
+  unfold ecfg_reg2 in *;
+  unfold ecfg_update_exp2 in *;
+  unfold ccfg_update_com2 in *;
+  unfold ccfg_update_mem2 in *;
+  unfold ccfg_update_mem in *;
+  unfold ccfg_update_reg in *;
+  unfold ccfg_update_com in *;
+  unfold ccfg_to_ecfg in *;
+  unfold project_ccfg.
+
+Section Preservation.
+  Lemma impe2_final_config_preservation (G: context) (d: loc_mode) :
+    forall G' c r m pc md r' m' t,
+      cstep2 md d (c,r,m) (r', m') t ->
+      cconfig2_ok pc md G d c r m G' ->
+      cterm2_ok G' d r' m'.
+  Proof.
+    intros G' c r m pc md r' m' t Hcstep Hcfgok.
+    remember (c,r,m) as ccfg.
+    remember (r',m') as cterm.
+    generalize dependent G.
+    generalize dependent G'.
+    generalize dependent pc.
+    generalize dependent c.
+    generalize dependent r.
+    generalize dependent m.
+    generalize dependent r'.
+    generalize dependent m'.
+    pose Hcstep as Hcstep'.
+    induction Hcstep'; unfold cterm2_ok; intros; subst; simpl in *; unfold_cfgs;
+      unfold cconfig2_ok in Hcfgok; destruct_pairs; unfold_cfgs; subst;
+        inversion Heqcterm; subst.
+    (* CSkip *)
+    - inversion H0; try discriminate; subst. split; [intros | split; intros]; simpl in *; auto.
+      -- now apply H1 in H.
+      -- now apply H2 in H.
+    (* CAssign *)
+    - inversion H1; try discriminate; subst.
+      split; [intros | split; intros]; simpl in *; auto; unfold_cfgs.
+      -- destruct (Nat.eq_dec x0 x).
+         --- rewrite <- (Nat.eqb_eq x0 x) in e0; rewrite e0 in H.
+             destruct_pairs.
+             assert (cterm2_ok G d r m') as Hcterm.
+             unfold cterm2_ok; auto.
+             pose (econfig2_pair_protected
+                     md G d e p r m' v v1 v2 s 
+                     H H7 H0 Hcterm)
+               as Heconfig.
+             inversion H6; subst.
+             now apply (join_protected_l p pc).
+         --- rewrite <- (Nat.eqb_neq x0 x) in n. rewrite n in H.
+             now apply H2 in H.
+      -- inversion Hcstep; subst; try discriminate; unfold_cfgs. now apply H3 in H.
+    (* Cdeclassify *)
+    - inversion H2; try discriminate; subst.
+      split; [intros | split; intros]; simpl in *; auto; unfold_cfgs.
+      -- destruct (Nat.eq_dec x0 x).
+         --- rewrite <- (Nat.eqb_eq x0 x) in e0; rewrite e0 in H.
+             destruct_pairs.
+             unfold mem_esc_hatch_ind in H6.
+             assert (is_escape_hatch e) as Heh by now unfold is_escape_hatch.
+             pose (H6 e Heh m') as Helocs.
+             Search (loc_in_exp).
+             assert (forall l, loc_in_exp e l -> exists v, m' l = VSingle v) as Hmsing.
+             intros. pose (Helocs l H10) as tmp; destruct tmp; destruct_pairs; subst.
+             rewrite <- H12; exists x1; auto.
+             destruct (same_mem_locs_evals_same_value
+                         e r m' md d G (Typ s p) v H8 H1 Heh Hmsing).
+             rewrite H in H10. discriminate.
+         --- rewrite <- (Nat.eqb_neq x0 x) in n. rewrite n in H.
+             now apply H3 in H.
+      -- now apply H4 in H.
+   (* Cupdate *)
+    - inversion H2; try discriminate; subst.
+      split; [intros | split; intros]; simpl in *; auto; unfold_cfgs; subst.
+      -- now apply H3 in H.
+      -- destruct (Nat.eq_dec l0 l).
+         --- pose e as e'. rewrite <- (Nat.eqb_eq l0 l) in e'; rewrite e' in H.
+             destruct_pairs.
+             pose (econfig2_pair_protected md G' d e2 p' r' m v v1 v2 s
+                                           H H9 H1) as Hprotected.
+             assert (cterm2_ok G' d r' m) as cterm2ok by now unfold cterm2_ok in *.
+             apply Hprotected in cterm2ok.
+             assert (p = p0) as peq. eapply ref_type. apply H2. apply H0. apply H8. apply H9.
+             rewrite e in H7; apply H7.
+             rewrite <- peq.
+             apply sec_level_join_le_l in H14. apply sec_level_join_le_l in H14.
+             inversion cterm2ok; subst. unfold sec_level_le in *.
+             destruct p0; auto; try omega.
+         --- rewrite <- (Nat.eqb_neq l0 l) in n. rewrite n in H.
+             now apply H4 in H.
+    (* Coutput *)
+    - inversion H1; try discriminate; subst; split; auto.
+    (* CCall *)
+    - inversion H1; try discriminate; subst.
+      unfold forall_dom in *; destruct_pairs.
+      assert (com_type pc md G d c G') as lifted_ctyp.
+      eapply subsumption; eauto.
+      eapply call_fxn_typ; eauto.
+      assert (estep md d (e,project_reg r true,project_mem m true) (Vlambda md c))
+        as estep2estep.
+      apply (impe2_exp_sound md d e r m (VSingle (Vlambda md c))); auto.
+      apply estep2estep.
+      now apply (sec_level_join_le_l pc q p).
+      
+      assert (cterm2_ok G' d r'0 m'0).
+      -- eapply (IHHcstep' Hcstep' m'0 r'0 Heqcterm m r c); auto.
+         unfold cconfig2_ok; split; eauto.
+      -- unfold cterm2_ok in *; destruct_pairs; auto.
+    (* Call-Div *)
+    - inversion H5; try discriminate; subst.
+      remember (VPair (Vlambda md c1) (Vlambda md c2)) as v.
+      assert (protected q) as qP.
+      eapply (econfig2_pair_protected md G d e q r m v
+                                      (Vlambda md c1) (Vlambda md c2)
+                                      (Tlambda Gm p md Gp)); eauto.
+      unfold cterm2_ok in *; auto.
+      assert (protected p) as pP. apply sec_level_join_le_r in H11. inversion qP; subst.
+      unfold sec_level_le in H11; destruct p; try omega; auto.
+      inversion pP; subst.
+
+      assert (com_type Common.H md G d c1 G') as lifted_c1typ.
+      eapply subsumption; eauto.
+      eapply call_fxn_typ; eauto.
+      assert (estep md d (e,project_reg r true,project_mem m true) (Vlambda md c1))
+        as estep2estep.
+      apply (impe2_exp_sound md d e r m (VPair (Vlambda md c1) (Vlambda md c2))); auto.
+      apply estep2estep.
+      destruct pc; unfold sec_level_le; auto.
+      assert (com_type Common.H md G d c2 G') as lifted_c2typ.
+      eapply subsumption; eauto.
+      eapply call_fxn_typ; eauto.
+      assert (estep md d (e,project_reg r false,project_mem m false) (Vlambda md c2))
+        as estep2estep.
+      apply (impe2_exp_sound md d e r m (VPair (Vlambda md c1) (Vlambda md c2))); auto.
+      apply estep2estep.
+      destruct pc; unfold sec_level_le; auto.
+
+      split; intros; destruct_pairs; subst.
+      (* see if there was an assignment in either c1 or c2 to change the registers *)
+      -- destruct (assign_in_dec c1 x), (assign_in_dec c2 x).
+         --- pose (assignment_more_secure Common.H md d c1 G G' x bt p lifted_c1typ a H14). 
+             destruct p. unfold sec_level_le in *. omega.
+             unfold protected; auto.
+         --- pose (assignment_more_secure Common.H md d c1 G G' x bt p lifted_c1typ a H14). 
+             destruct p. unfold sec_level_le in *. omega.
+             unfold protected; auto.
+         --- pose (assignment_more_secure Common.H md d c2 G G' x bt p lifted_c2typ a H14). 
+             destruct p. unfold sec_level_le in *. omega.
+             unfold protected; auto.
+         --- pose (no_assign_reg_context_constant
+                     md d (Ccall e) r m r' m' (merge_trace (t1, t2)) x pc G G' Hcstep H5).
+             assert (~assign_in (Ccall e) x) as noassign.
+             rewrite (assign_not_in_call_div e x md d r m c1 c2); split; auto.
+             apply a in noassign; destruct_pairs.
+             apply (H6 x v1 v2 bt p). split. rewrite H15; auto. rewrite H16; auto.
+      -- split; auto. intros; destruct_pairs.
+         destruct (update_in_dec c1 l), (update_in_dec c2 l).
+         --- pose (update_more_secure Common.H md d c1 G G' l bt p rt lifted_c1typ u H14). 
+             destruct p. unfold sec_level_le in *. omega.
+             unfold protected; auto.
+         --- pose (update_more_secure Common.H md d c1 G G' l bt p rt lifted_c1typ u H14). 
+             destruct p. unfold sec_level_le in *. omega.
+             unfold protected; auto.
+         --- pose (update_more_secure Common.H md d c2 G G' l bt p rt lifted_c2typ u H14). 
+             destruct p. unfold sec_level_le in *. omega.
+             unfold protected; auto.
+         --- pose (no_update_mem_constant
+                     md d (Ccall e) r m r' m' (merge_trace (t1, t2)) l pc G G' Hcstep H5).
+             assert (~update_in (Ccall e) l) as noupdate.
+             rewrite (update_not_in_call_div e l md d r m c1 c2); split; auto.
+             apply e0 in noupdate.
+             apply (H7 l v1 v2 bt p rt). split; auto. rewrite noupdate; auto. 
+    (* Cenclave *)
+    - inversion H; try discriminate; subst. inversion H0; subst.
+      eapply IHHcstep'; auto.
+      unfold cconfig2_ok; auto; split.
+      apply H5.  split; auto.
+    (* Cseq-Nil*)
+    - inversion H0; try discriminate; subst; split; auto.
+    (* Cseq *)
+    - inversion H0; try discriminate; subst.
+      assert (cconfig2_ok pc md G d hd r0 m0 g') as hdcfg_ok.
+      unfold cconfig2_ok; eauto.
+      
+      assert (cterm2_ok g' d r m) as hdcterm2_ok.
+      eapply IHHcstep'1; eauto.
+      unfold cterm2_ok in *; destruct_pairs.
+      
+      assert (cterm2_ok G' d r'0 m'0) as tl_cterm2_ok.
+      eapply (IHHcstep'2 Hcstep'2 m'0 r'0 Heqcterm m r (Cseq tl)); eauto.
+      unfold cconfig2_ok; eauto.
+      unfold cterm2_ok in *; now destruct_pairs.
+    (* Cif *)
+    - inversion H1; try discriminate; subst.
+      eapply IHHcstep'; auto.
+      assert (cconfig2_ok pc' md G d c1 r m G') as c1ok.
+      unfold cconfig2_ok; split; auto.
+      apply c1ok.
+    (* Celse *)
+    - inversion H1; try discriminate; subst.
+      eapply IHHcstep'; auto.
+      assert (cconfig2_ok pc' md G d c2 r m G') as c2ok.
+      unfold cconfig2_ok; split; auto.
+      apply c2ok.
+    (* Cif-Div *)
+    - inversion H6; try discriminate; subst.
+      assert (protected p).
+      remember (VPair (Vnat n1) (Vnat n2)) as v.
+      eapply econfig2_pair_protected. apply Heqv. apply H20. apply H0.
+      assert (cterm2_ok G d r m) as Hcterm2_ok.
+      unfold cterm2_ok in *; auto.
+      apply Hcterm2_ok.
+      (* get that pc' is protected *)
+      assert (protected (sec_level_join pc p)) by now apply (join_protected_r pc p).
+      inversion H12; subst. rewrite H16 in H22.
+      destruct pc'; unfold sec_level_le in H22. omega.
+      clear H22 H H12 H16.
+      split; intros; destruct_pairs.
+      (* see if there was an assignment in either c1 or c2 to change the registers *)
+      -- destruct (assign_in_dec c1 x), (assign_in_dec c2 x).
+         --- pose (assignment_more_secure Common.H md d c1 G G' x bt p0 H14 a H12).
+             destruct p0. unfold sec_level_le in *. omega.
+             unfold protected; auto.
+         --- pose (assignment_more_secure Common.H md d c1 G G' x bt p0 H14 a H12).
+             destruct p0. unfold sec_level_le in *. omega.
+             unfold protected; auto.
+         --- pose (assignment_more_secure Common.H md d c2 G G' x bt p0 H15 a H12).
+             destruct p0. unfold sec_level_le in *. omega.
+             unfold protected; auto.
+         --- pose (no_assign_reg_context_constant
+                     md d (Cif e c1 c2) r m r' m' (merge_trace (t1, t2)) x pc G G'
+                     Hcstep H6).
+             assert (~ assign_in (Cif e c1 c2) x) as noassign.
+             rewrite (assign_in_if_else e c1 c2 x). apply and_not_or. split; auto.
+             apply a in noassign; destruct_pairs.
+             apply (H7 x v1 v2 bt p0). split. rewrite H13; auto. rewrite H16; auto.
+      -- split; auto. intros; destruct_pairs.
+         destruct (update_in_dec c1 l), (update_in_dec c2 l).
+         --- pose (update_more_secure Common.H md d c1 G G' l bt p0 rt H14 u H12).
+             destruct p0. unfold sec_level_le in *. omega.
+             unfold protected; auto.
+         --- pose (update_more_secure Common.H md d c1 G G' l bt p0 rt H14 u H12).
+             destruct p0. unfold sec_level_le in *. omega.
+             unfold protected; auto.
+         --- pose (update_more_secure Common.H md d c2 G G' l bt p0 rt H15 u H12).
+             destruct p0. unfold sec_level_le in *. omega.
+             unfold protected; auto.
+         --- pose (no_update_mem_constant
+                     md d (Cif e c1 c2) r m r' m' (merge_trace (t1, t2)) l pc G G'
+                     Hcstep H6).
+             assert (~ update_in (Cif e c1 c2) l) as noupdate.
+             rewrite (update_in_if_else e c1 c2 l). apply and_not_or. split; auto.
+             apply e0 in noupdate; destruct_pairs.
+             apply (H8 l v1 v2 bt p0 rt). split; [rewrite noupdate | ]; auto. 
+    (* Cwhile-T *)
+    - inversion H1; try discriminate; subst.
+      (* cterm after executing c is ok *)
+      assert (cterm2_ok G' d r m) as cok.
+      eapply IHHcstep'1; auto.
+      assert (cconfig2_ok pc' md G' d c r0 m0 G') as ccfgok.
+      unfold cconfig2_ok in *; split; auto.
+      apply ccfgok.
+      (* cterm after executing the rest of while is ok *)
+      assert (cterm2_ok G' d r'0 m'0).
+      eapply IHHcstep'2; auto.
+      assert (cconfig2_ok pc md G' d (Cwhile e c) r m G') as cwhileok.
+      unfold cterm2_ok in *; destruct_pairs; unfold cconfig2_ok in *; split; auto.
+      apply cwhileok.
+      (* putting them together, final state is ok *)
+      unfold cterm2_ok in *; destruct_pairs. split; auto.
+    (* Cwhile-F *)
+    - inversion H1; try discriminate; subst. auto.
+    (* Cwhile-Div *)
+    - inversion H6; try discriminate; subst.
+      assert (protected p).
+      remember (VPair (Vnat n1) (Vnat n2)) as v.
+      eapply econfig2_pair_protected. apply Heqv. apply H13. apply H0.
+      assert (cterm2_ok G' d r m) as Hcterm2_ok.
+      unfold cterm2_ok in *; auto.
+      apply Hcterm2_ok.
+      (* get that pc' is protected *)
+      assert (protected (sec_level_join pc p)) by now apply (join_protected_r pc p).
+      inversion H12; subst. rewrite H16 in H19.
+      destruct pc'; unfold sec_level_le in H19. omega.
+      split; intros; destruct_pairs.
+      (* see if there was an assignment in c to change the registers *)
+      -- destruct (assign_in_dec c x).
+         --- pose (assignment_more_secure Common.H md d c G' G' x bt p0 H14 a H17).
+             destruct p0. unfold sec_level_le in *. omega.
+             unfold protected; auto.
+         --- pose (no_assign_reg_context_constant
+                     md d (Cwhile e c) r m r' m' (merge_trace (t1, t2)) x pc G' G'
+                     Hcstep H6).
+             assert (~assign_in (Cwhile e c) x) as noassign by
+                   now rewrite (assign_in_while e c x).
+             apply a in noassign; destruct_pairs.
+             apply (H7 x v1 v2 bt p0). split; auto. rewrite H18; auto.
+      -- split; auto. intros; destruct_pairs.
+         destruct (update_in_dec c l).
+         --- pose (update_more_secure Common.H md d c G' G' l bt p0 rt H14 u H17).
+             destruct p0. unfold sec_level_le in *. omega.
+             unfold protected; auto.
+         --- pose (no_update_mem_constant
+                     md d (Cwhile e c) r m r' m' (merge_trace (t1, t2)) l pc G' G'
+                     Hcstep H6).
+             assert (~update_in (Cwhile e c) l) as noupdate by
+                   now rewrite (update_in_while e c l).
+             apply e0 in noupdate; destruct_pairs.
+             apply (H8 l v1 v2 bt p0 rt). split; auto. rewrite noupdate; auto.
+  Qed.
+
+  Lemma impe2_type_preservation 
+        (G: context) (d: loc_mode) :
+    forall pc md c r m G' mdmid cmid rmid mmid rmid' mmid' tmid rfin mfin tfin,
+      cconfig2_ok pc md G d c r m G' ->
+      cstep2 mdmid d (cmid, rmid, mmid) (rmid', mmid') tmid
+      -> cstep2 md d (c, r, m) (rfin, mfin) tfin
+      -> imm_premise cmid mdmid rmid mmid rmid' mmid' tmid
+                     c md r m rfin mfin tfin d ->
+      exists pcmid Gmid Gmid',
+        sec_level_le pc pcmid /\ cconfig2_ok pcmid mdmid Gmid d cmid rmid mmid Gmid'.
+  Proof.
+    intros pc md c r m G' mdmid cmid rmid mmid rmid' mmid' tmid rfin mfin tfin
+           Hccfg2ok HIP.
+    revert tfin mfin rfin tmid mmid' rmid' mmid rmid cmid mdmid r m G' Hccfg2ok HIP.
+    induction c; intros; destruct_pairs; inversion H0; try discriminate; subst; unfold_cfgs;
+      inversion Hccfg2ok; try discriminate; subst; destruct_pairs;
+        inversion H1; try discriminate; subst; unfold_cfgs.
+    (* CALL *)
+    - exists p. exists Gm. exists Gp. split. now apply sec_level_join_le_l in H10.
+      unfold cconfig2_ok; split; auto; unfold_cfgs.
+      eapply call_fxn_typ; eauto. 
+      assert (estep md d (e,project_reg r true,project_mem m true) (Vlambda md cmid))
+        as estep2estep.
+      apply (impe2_exp_sound md d e r m (VSingle (Vlambda md cmid))); auto.
+      apply estep2estep.
+      split; auto; intros; unfold forall_dom in *; destruct_pairs.
+      inversion H12; subst.
+      -- apply H16 in H14; destruct H14; destruct_pairs.
+         inversion H17; subst.
+         assert (protected p1) by now apply (H4 x v1 v2 s1 p1).
+         inversion H19; subst. 
+         destruct p0; unfold sec_level_le in *; auto; try omega.
+    (* ENCLAVE *)
+    - exists pc. exists G. exists G'. split. apply sec_level_le_refl.
+      split. inversion Hccfg2ok; unfold_cfgs; subst; try discriminate; destruct_pairs.
+      inversion H1; try discriminate; unfold_cfgs; subst. inversion H6; subst.
+      inversion H15; subst; auto.
+      unfold cconfig2_ok; split; unfold_cfgs; auto.
+    (* SEQ1 *)
+    - exists pc. exists G. exists g'.
+      split. apply sec_level_le_refl.
+      split. auto.
+      unfold cconfig2_ok; split; unfold_cfgs; auto.
+    (* SEQ2 *)
+    - exists pc. exists g'. exists G'.
+      split. apply sec_level_le_refl.
+      assert (cconfig2_ok pc md G d c r m g') as c_ok.
+      unfold cconfig2_ok in *; destruct_pairs.
+      split; auto. 
+      assert (cterm2_ok g' d rmid mmid) as cterm2ok.
+      apply (impe2_final_config_preservation G d g' c r m pc md rmid mmid tr'); auto.
+      unfold cconfig2_ok in *; unfold cterm2_ok in *; destruct_pairs; unfold_cfgs; auto.
+    (* IF *)
+    - exists pc'. exists G. exists G'.
+      split. now apply (sec_level_join_le_l pc p pc') in H19.
+      split; unfold cconfig2_ok; auto.
+    (* ELSE *)
+    - exists pc'. exists G. exists G'.
+      split. now apply (sec_level_join_le_l pc p pc') in H18.
+      split; unfold cconfig2_ok; auto.
+    (* WHILE1 *)
+    - exists pc'. exists G'. exists G'.
+      split. now apply (sec_level_join_le_l pc p pc') in H17.
+      split; unfold cconfig2_ok; auto.
+    (* WHILE2 *)
+    - exists pc. exists G'. exists G'.
+      split. now apply sec_level_le_refl.
+      split; auto.
+      assert (cconfig2_ok pc' md G' d c r m G').
+      unfold cconfig2_ok; split; unfold_cfgs; auto.
+      assert (cterm2_ok G' d rmid mmid) as cterm2ok.
+      apply (impe2_final_config_preservation G' d G' c r m pc' md rmid mmid tr'); auto.
+      unfold cconfig2_ok in *; unfold cterm2_ok in *; destruct_pairs; unfold_cfgs; auto.
+  Qed.
+  
+End Preservation.
+
+(*******************************************************************************
+*
+* SECURITY_PASSIVE
+*
+*******************************************************************************)
+
+Section Secure_Passive.
+  Lemma config2_ok_implies_obs_equal (m: mem2) (c: com) (t: trace2) :
+    forall pc md G d r G' r' m',
+      cconfig2_ok pc md G d c r m G' ->
+      cstep2 md d (c,r,m) (r',m') t ->
+      tobs_sec_level L (project_trace t true) = tobs_sec_level L (project_trace t false).
+  Proof.
+    intros pc md G d r G' r' m' Hccfg2ok Hcstep2.
+    remember (c,r,m) as ccfg.
+    generalize dependent c.
+    generalize dependent r.
+    generalize dependent m.
+    generalize dependent pc.
+    generalize dependent G'.
+    generalize dependent G.
+    pose Hcstep2 as Hcstep.
+    induction Hcstep; intros; subst; simpl in *; auto; repeat unfold_cfgs; subst.
+    (* OUTPUT *)
+    - unfold sec_level_le_compute. destruct sl; auto.
+      destruct v; simpl; auto.
+      inversion Hccfg2ok; destruct_pairs; unfold_cfgs; subst; auto; try discriminate.
+      inversion H; unfold_cfgs; try discriminate; subst; auto.
+      remember (VPair v v0) as vpair.
+      assert (cterm2_ok G' d r m) as Hctermok; unfold cterm2_ok; auto.
+      assert (protected p) by apply (econfig2_pair_protected
+                                       md G' d e p r m vpair v v0 s
+                                       Heqvpair H11 H0 Hctermok).
+      pose (sec_level_join_ge p pc); destruct_pairs.
+      apply (sec_level_le_trans p (sec_level_join p pc) L) in H13; auto.
+      destruct p; inversion H5; inversion H13.
+    (* CALL *)
+    - assert (imm_premise c md r m r'0 m'0 tr
+                          (Ccall e) md r m r'0 m'0 tr d)
+        as HIP by now apply IPcall.
+      pose (impe2_type_preservation G d pc md (Ccall e) r m G'
+                                    md c r m r'0 m'0 tr r'0 m'0 tr 
+                                    Hccfg2ok Hcstep Hcstep2 HIP)
+        as Lemma6.
+      destruct Lemma6 as [pcmid [Gmid [Gmid' Lemma6]]]; destruct_pairs; subst.
+      apply (IHHcstep Hcstep Gmid Gmid' pcmid m r c H1); auto.
+    (* CALL-DIV *)
+    - remember (VPair (Vlambda md c1) (Vlambda md c2)) as v.
+      inversion Hccfg2ok; destruct_pairs; unfold_cfgs; subst; auto; try discriminate.
+      inversion H; unfold_cfgs; try discriminate; subst; auto.
+      assert (protected q) as Hqprotected.
+      eapply econfig2_pair_protected in H10; auto. apply H0.
+      assert (cterm2_ok G d r m) by now unfold cterm2_ok. apply H9.
+      assert (protected (sec_level_join pc q)) as Hpcqprotected
+          by apply (join_protected_r pc q Hqprotected).
+      inversion Hpcqprotected; rewrite Hpcqprotected in H11.
+      assert (protected p) as Hpprotected.
+      unfold protected. unfold sec_level_le in H11; destruct p; intuition.
+      clear H11 H14.
+      assert (com_type p md Gm d c1 Gp).
+      eapply call_fxn_typ; eauto. 
+      assert (estep md d (e,project_reg r true,project_mem m true) (Vlambda md c1))
+        as estepc1.
+      apply (impe2_exp_sound md d e r m (VPair (Vlambda md c1) (Vlambda md c2))); auto.
+      apply estepc1.
+      assert (com_type p md Gm d c2 Gp).
+      eapply call_fxn_typ; eauto. 
+      assert (estep md d (e,project_reg r false,project_mem m false) (Vlambda md c2))
+        as estepc2.
+      apply (impe2_exp_sound md d e r m (VPair (Vlambda md c1) (Vlambda md c2))); auto.
+      apply estepc2.
+      assert (tobs_sec_level L t1 = []) as t1_empty.
+      eapply protected_typ_no_obs_output in H1; auto.
+      apply H9; auto. auto.
+      assert (tobs_sec_level L t2 = []) as t2_empty.
+      eapply protected_typ_no_obs_output in H2; auto.
+      apply H11; auto. auto.
+      pose (project_merge_inv_trace t1 t2 true) as Ht1; simpl in *.
+      pose (project_merge_inv_trace t1 t2 false) as Ht2; simpl in *.
+      now rewrite Ht1, Ht2, t1_empty, t2_empty.
+    (* ENCLAVE *)
+    - assert (imm_premise c (Encl enc) r m r'0 m'0 tr
+                          (Cenclave enc c) Normal r m r'0 m'0 tr d)
+        as HIP by now apply IPencl.
+      pose (impe2_type_preservation G d pc Normal (Cenclave enc c) r m G'
+                                    (Encl enc) c r m r'0 m'0 tr _ _ _ 
+                                    Hccfg2ok Hcstep Hcstep2 HIP) as Lemma6.
+      destruct Lemma6 as [pcmid [Gmid [Gmid' Lemma6]]]; destruct_pairs; subst.
+      apply (IHHcstep Hcstep Gmid Gmid' pcmid m r c H0); auto.
+   (* SEQ *)
+    - assert (imm_premise hd md r0 m0 r m tr
+                          (Cseq (hd::tl)) md r0 m0 r'0 m'0 (tr++tr') d)
+        as HIP1 by apply (IPseq1 _ _ _ _ _ _ _ _ _ _ _ _ Hcstep1 Hcstep3 Hcstep2).
+      pose (impe2_type_preservation G d pc md (Cseq (hd::tl)) r0 m0 G'
+                                    md hd r0 m0 r m tr _ _ _ 
+                                    Hccfg2ok Hcstep1 Hcstep2 HIP1) as Lemma61.
+
+      assert (imm_premise (Cseq tl) md r m r'0 m'0 tr'
+                          (Cseq (hd::tl)) md r0 m0 r'0 m'0 (tr++tr') d)
+        as HIP2 by apply (IPseq2 _ _ _ _ _ _ _ _ _ _ _ _ Hcstep1 Hcstep3 Hcstep2).
+      pose (impe2_type_preservation G d pc md (Cseq (hd::tl)) r0 m0 G'
+                                    md (Cseq tl) r m r'0 m'0 tr' _ _ _
+                                    Hccfg2ok Hcstep3 Hcstep2 HIP2)
+        as Lemma62.
+
+      destruct Lemma61 as [pcmid1 [Gmid1 [Gmid1' Lemma6]]]; destruct_pairs; subst.
+      destruct Lemma62 as [pcmid2 [Gmid2 [Gmid2' Lemma6]]]; destruct_pairs; subst.
+      assert (cconfig2_ok pcmid1 md Gmid1 d hd r0 m0 Gmid1') as seq1OK by now auto.
+      assert (cconfig2_ok pcmid2 md Gmid2 d (Cseq tl) r m Gmid2') as seq2OK by now auto.
+      pose (IHHcstep1 Hcstep1 Gmid1 Gmid1' pcmid1 m0 r0 hd seq1OK) as tr_same.
+      pose (IHHcstep2 Hcstep3 Gmid2 Gmid2' pcmid2 m r (Cseq tl) seq2OK) as tr'_same.
+      rewrite project_app_trace.
+      rewrite <- tobs_sec_level_app.
+      rewrite tr'_same, tr_same; auto.
+      rewrite tobs_sec_level_app. rewrite project_app_trace; auto.
+    (* IF *)
+    -  assert (imm_premise c1 md r m r'0 m'0 tr
+                           (Cif e c1 c2) md r m r'0 m'0 tr d)
+         as HIP by apply (IPif  _ _ _ _ _ _ _ _ _ _ H0 Hcstep Hcstep2 Hcstep2).
+       pose (impe2_type_preservation G d pc md (Cif e c1 c2) r m G'
+                                     md c1 r m r'0 m'0 tr _ _ _
+                                     Hccfg2ok Hcstep Hcstep2 HIP) as Lemma6.
+       destruct Lemma6 as [pcmid [Gmid [Gmid' Lemma6]]]; destruct_pairs; subst.
+       apply (IHHcstep Hcstep Gmid Gmid' pcmid m r c1 H1); auto.
+    (* ELSE *)
+    -  assert (imm_premise c2 md r m r'0 m'0 tr
+                           (Cif e c1 c2) md r m r'0 m'0 tr d)
+         as HIP by apply (IPelse _ _ _ _ _ _ _ _ _ _ H0 Hcstep Hcstep2).
+       pose (impe2_type_preservation G d pc md (Cif e c1 c2) r m G'
+                                     md c2 r m r'0 m'0 tr _ _ _
+                                     Hccfg2ok Hcstep Hcstep2 HIP) as Lemma6.
+       destruct Lemma6 as [pcmid [Gmid [Gmid' Lemma6]]]; destruct_pairs; subst.
+       apply (IHHcstep Hcstep Gmid Gmid' pcmid m r c2 H1); auto.
+    (* IFELSE-DIV *)
+    - remember (VPair (Vnat n1) (Vnat n2)) as v.
+      inversion Hccfg2ok; destruct_pairs; unfold_cfgs; subst; auto; try discriminate.
+      inversion H; unfold_cfgs; try discriminate; subst; auto.
+      assert (protected p) as Hqprotected.
+      eapply econfig2_pair_protected in H20; auto. apply H0.
+      assert (cterm2_ok G d r m) by now unfold cterm2_ok. apply H11.
+      assert (protected (sec_level_join pc p)) by now apply (join_protected_r pc p).
+      inversion H11; rewrite H11 in H22.
+      assert (protected pc') as Hpc'protected.
+      unfold protected. unfold sec_level_le in H22. destruct pc'; intuition.
+      assert (tobs_sec_level L t1 = [] /\ tobs_sec_level L t2 = []).
+      destruct n1, n2; simpl in *;
+        eapply (protected_typ_no_obs_output r m) in H2;
+        eapply (protected_typ_no_obs_output r m) in H3;
+        try apply H14; try apply H15; auto.
+      destruct_pairs.
+      pose (project_merge_inv_trace t1 t2 true) as Ht1; simpl in *.
+      pose (project_merge_inv_trace t1 t2 false) as Ht2; simpl in *.
+      now rewrite Ht1, Ht2, H12, H16.
+    (* WHILE *)
+    - assert (imm_premise c md r0 m0 r m tr
+                          (Cwhile e c) md r0 m0 r'0 m'0 (tr++tr') d)
+        as HIP1 by apply (IPwhilet1 _ _ _ _ _ _ _ _ _ _ _ _ H0 Hcstep1 Hcstep3 Hcstep2).
+      pose (impe2_type_preservation G d pc md (Cwhile e c) r0 m0 G'
+                                    md c r0 m0 r m tr _ _ _ 
+                                    Hccfg2ok Hcstep1 Hcstep2 HIP1) as Lemma61.
+
+      assert (imm_premise (Cwhile e c) md r m r'0 m'0 tr'
+                          (Cwhile e c) md r0 m0 r'0 m'0 (tr++tr') d)
+        as HIP2 by apply (IPwhilet2 _ _ _ _ _ _ _ _ _ _ _ _ H0 Hcstep1 Hcstep3 Hcstep2).
+      pose (impe2_type_preservation G d pc md (Cwhile e c) r0 m0 G'
+                                    md (Cwhile e c) r m r'0 m'0 tr' _ _ _
+                                    Hccfg2ok Hcstep3 Hcstep2 HIP2)
+        as Lemma62.
+
+      destruct Lemma61 as [pcmid1 [Gmid1 [Gmid1' Lemma6]]]; destruct_pairs; subst.
+      destruct Lemma62 as [pcmid2 [Gmid2 [Gmid2' Lemma6]]]; destruct_pairs; subst.
+      assert (cconfig2_ok pcmid1 md Gmid1 d c r0 m0 Gmid1') as seq1OK by auto.
+      assert (cconfig2_ok pcmid2 md Gmid2 d (Cwhile e c) r m Gmid2') as seq2OK by auto.
+      pose (IHHcstep1 Hcstep1 Gmid1 Gmid1' pcmid1 m0 r0 c seq1OK) as tr_same.
+      pose (IHHcstep2 Hcstep3 Gmid2 Gmid2' pcmid2 m r (Cwhile e c) seq2OK) as tr'_same.
+      rewrite project_app_trace.
+      rewrite <- tobs_sec_level_app.
+      rewrite tr'_same, tr_same; auto.
+      rewrite tobs_sec_level_app. rewrite <- project_app_trace; auto.
+    (* WHILE-DIV *)
+    - remember (VPair (Vnat n1) (Vnat n2)) as v.
+      inversion Hccfg2ok; destruct_pairs; unfold_cfgs; subst; auto; try discriminate.
+      inversion H; unfold_cfgs; try discriminate; subst; auto.
+      assert (protected p) as Hqprotected.
+      eapply econfig2_pair_protected in H13; auto. apply H0.
+      assert (cterm2_ok G' d r m) by now unfold cterm2_ok. apply H11.
+      assert (protected (sec_level_join pc p)) by now apply (join_protected_r pc p).
+      inversion H11; rewrite H11 in H19.
+      assert (protected pc') as Hpc'protected.
+      unfold protected. unfold sec_level_le in H19. destruct pc'; intuition.
+
+      assert (com_type pc' md G' d Cskip G') as skip_typ by apply CTskip.
+      assert (com_type pc md G' d (Cseq [c; Cwhile e c]) G') as seq_type.
+      assert (com_type pc md G' d c G') as c_typ.
+      apply (subsumption pc' pc md d G' G' G' G' c) in H14; auto.
+      destruct pc; simpl in *; auto.
+      apply (context_le_refl G'). apply (context_le_refl G').
+      eapply Tseq. apply c_typ.
+      eapply Tseq. apply H.
+      eapply Tseqnil.
+      assert (tobs_sec_level L t1 = [] /\ tobs_sec_level L t2 = []).
+      destruct n1, n2; simpl in *.
+      -- eapply protected_typ_no_obs_output in H2; auto. 
+         eapply protected_typ_no_obs_output in H3; auto.
+         apply skip_typ. auto.
+         apply skip_typ. auto.
+      -- eapply protected_typ_no_obs_output in H2; auto. 
+         eapply protected_while_no_obs_output in H3; auto.
+         apply H. apply H14. auto.
+         apply skip_typ. auto.
+      -- eapply protected_while_no_obs_output in H2; auto.
+         eapply protected_typ_no_obs_output in H3; auto.
+         apply skip_typ. auto.
+         apply H. apply H14. auto.
+      -- eapply protected_while_no_obs_output in H2; auto.
+         eapply protected_while_no_obs_output in H3; auto.
+         apply H. apply H14; auto.
+         auto. apply H. apply H14. auto.
+      -- destruct_pairs.
+         pose (project_merge_inv_trace t1 t2 true) as Ht1; simpl in *.
+         pose (project_merge_inv_trace t1 t2 false) as Ht2; simpl in *.
+         now rewrite Ht1, Ht2, H12, H16.
+  Qed.
+ 
+  Lemma secure_passive : forall G G' d c,
+    well_formed_spec g0 ->
+    corresponds G ->
+    com_type L Normal G d c G' ->
+    secure_prog L d c G.
+  Proof.
+    unfold secure_prog.
+    intros G G' d c Hg0wf Hcorr Hcomtype
+           m0 mknown r' m' t tobs Hmmerge
+           Hcstep2 Htobs Hind Hesc.
+    rewrite Htobs.
+    apply (config2_ok_implies_obs_equal minit c t (L) Normal G d
+                     reg_init2 G' r' m'); auto.
+    unfold cconfig2_ok; split; unfold_cfgs; auto.
+    split; intros; destruct_pairs.
+    - inversion H.
+    - split; intros; destruct_pairs.
+      -- unfold corresponds in Hcorr; destruct_pairs.
+         unfold well_formed_spec in Hg0wf.
+         pose (Hg0wf l) as Hgwf; destruct Hgwf; destruct_pairs.
+         pose H3 as Hg0. apply (H1 l x bt rt) in Hg0.
+         rewrite H0 in Hg0. inversion Hg0; subst.
+         apply (diff_loc_protected l); auto.
+         apply (vpair_if_diff m0 mknown v1 v2 l) in H; auto.
+         apply project_merge_inv_mem in Hmmerge; destruct_pairs; subst; auto.
+      -- split; intros; auto.
+  Qed.
+End Secure_Passive.
